<?xml version="1.0"?>


<!DOCTYPE rdf:RDF [
    <!ENTITY owl "http://www.w3.org/2002/07/owl#" >
    <!ENTITY dc "http://purl.org/dc/elements/1.1/" >
    <!ENTITY xsd "http://www.w3.org/2001/XMLSchema#" >
    <!ENTITY rdfs "http://www.w3.org/2000/01/rdf-schema#" >
    <!ENTITY rdf "http://www.w3.org/1999/02/22-rdf-syntax-ns#" >
    <!ENTITY dataquality "http://www.semanticweb.org/ontologies/dataquality.owl#" >
    <!ENTITY dataqualitymodule "http://www.semanticweb.org/ontologies/dataqualitymodule.owl#" >
]>


<rdf:RDF xmlns="http://wsmls.googlecode.com/svn/trunk/global/Patterns/Quality/DataQuality/servicequalitymodule.owl#"
     xml:base="http://wsmls.googlecode.com/svn/trunk/global/Patterns/Quality/DataQuality/servicequalitymodule.owl"
     xmlns:dc="http://purl.org/dc/elements/1.1/"
     xmlns:rdfs="http://www.w3.org/2000/01/rdf-schema#"
     xmlns:dataquality="http://www.semanticweb.org/ontologies/dataquality.owl#"
     xmlns:owl="http://www.w3.org/2002/07/owl#"
     xmlns:xsd="http://www.w3.org/2001/XMLSchema#"
     xmlns:rdf="http://www.w3.org/1999/02/22-rdf-syntax-ns#"
     xmlns:dataqualitymodule="http://www.semanticweb.org/ontologies/dataqualitymodule.owl#">
    <owl:Ontology rdf:about="http://wsmls.googlecode.com/svn/trunk/global/Patterns/Quality/DataQuality/servicequalitymodule.owl">
        <dc:date>July 31, 2012</dc:date>
        <rdfs:comment>The concepts suggested in this module are not aligned to a foundational ontology because the goal is to provide a simple and readily re-usable set of concepts for semantic annotation. The module aligned to the foundational ontology Dolce Ultra Light (DUL) can be accessed at http://ifgi.uni-muenster.de/~degbelo/Ressources/SSN2012Degbelo. The module is similar to the &#39;Ontology design pattern for spatial data quality characterization in the Semantic Sensor Web&#39;.</rdfs:comment>
        <dc:contributor>Auriol Degbelo &lt;degbelo@uni-muenster.de&gt;</dc:contributor>
        <dc:title>An ontology design pattern for (web) service quality characterization in the Semantic Sensor Web.</dc:title>
    </owl:Ontology>
    


    <!-- 
    ///////////////////////////////////////////////////////////////////////////////////////
    //
    // Annotation properties
    //
    ///////////////////////////////////////////////////////////////////////////////////////
     -->

    <owl:AnnotationProperty rdf:about="&dc;contributor"/>
    <owl:AnnotationProperty rdf:about="&dc;date"/>
    <owl:AnnotationProperty rdf:about="&rdfs;comment"/>
    <owl:AnnotationProperty rdf:about="&dc;title"/>
    


    <!-- 
    ///////////////////////////////////////////////////////////////////////////////////////
    //
    // Object Properties
    //
    ///////////////////////////////////////////////////////////////////////////////////////
     -->

    


    <!-- http://www.semanticweb.org/ontologies/dataquality.owl#approximates -->

    <owl:ObjectProperty rdf:about="&dataquality;approximates">
        <rdfs:comment>a relation between a service quality assessment operation and the service quality component that is assessed.</rdfs:comment>
        <rdfs:range rdf:resource="&dataquality;ServiceQualityComponent"/>
        <rdfs:domain rdf:resource="&dataquality;ServiceQualityObservation"/>
        <owl:inverseOf rdf:resource="&dataqualitymodule;isApproximatedBy"/>
        <rdfs:subPropertyOf rdf:resource="&owl;topObjectProperty"/>
    </owl:ObjectProperty>
    


    <!-- http://www.semanticweb.org/ontologies/dataquality.owl#involves -->

    <owl:ObjectProperty rdf:about="&dataquality;involves">
        <rdfs:comment>this property relates a service quality assessment operation to the result of the operation.</rdfs:comment>
        <rdfs:domain rdf:resource="&dataquality;ServiceQualityObservation"/>
        <rdfs:range rdf:resource="&dataquality;ServiceQualityResult"/>
        <rdfs:subPropertyOf rdf:resource="&owl;topObjectProperty"/>
    </owl:ObjectProperty>
    


    <!-- http://www.semanticweb.org/ontologies/dataquality.owl#isQualityComponentOf -->

    <owl:ObjectProperty rdf:about="&dataquality;isQualityComponentOf">
        <rdfs:comment>a relation between a component of web service quality (e.g. reliability, robustness) and the web service.</rdfs:comment>
        <rdfs:range rdf:resource="&dataquality;Service"/>
        <rdfs:domain rdf:resource="&dataquality;ServiceQualityComponent"/>
        <rdfs:subPropertyOf rdf:resource="&owl;topObjectProperty"/>
    </owl:ObjectProperty>
    


    <!-- http://www.semanticweb.org/ontologies/dataquality.owl#satisfies -->

    <owl:ObjectProperty rdf:about="&dataquality;satisfies">
        <rdfs:comment>a service quality assessment should conform to a criterion defined by the web service consumer. This property makes explicit the criterion used while assigning a value to a service quality component.</rdfs:comment>
        <rdfs:range rdf:resource="&dataquality;ServiceQualityCriterion"/>
        <rdfs:domain rdf:resource="&dataquality;ServiceQualityObservation"/>
        <owl:inverseOf rdf:resource="&dataqualitymodule;isQualityCriterionOf"/>
        <rdfs:subPropertyOf rdf:resource="&owl;topObjectProperty"/>
    </owl:ObjectProperty>
    


    <!-- http://www.semanticweb.org/ontologies/dataqualitymodule.owl#hasQualityComponent -->

    <owl:ObjectProperty rdf:about="&dataqualitymodule;hasQualityComponent">
        <rdfs:comment>inverse property of &#39;isPropertyOf&#39;.</rdfs:comment>
        <owl:inverseOf rdf:resource="&dataquality;isQualityComponentOf"/>
        <rdfs:subPropertyOf rdf:resource="&owl;topObjectProperty"/>
    </owl:ObjectProperty>
    


    <!-- http://www.semanticweb.org/ontologies/dataqualitymodule.owl#isApproximatedBy -->

    <owl:ObjectProperty rdf:about="&dataqualitymodule;isApproximatedBy">
        <rdfs:comment>inverse property of &#39;approximates&#39;.</rdfs:comment>
        <rdfs:subPropertyOf rdf:resource="&owl;topObjectProperty"/>
    </owl:ObjectProperty>
    


    <!-- http://www.semanticweb.org/ontologies/dataqualitymodule.owl#isQualityCriterionOf -->

    <owl:ObjectProperty rdf:about="&dataqualitymodule;isQualityCriterionOf">
        <rdfs:comment>inverse property of &#39;satisfies&#39;.</rdfs:comment>
        <rdfs:subPropertyOf rdf:resource="&owl;topObjectProperty"/>
    </owl:ObjectProperty>
    


    <!-- http://www.semanticweb.org/ontologies/dataqualitymodule.owl#isResultOf -->

    <owl:ObjectProperty rdf:about="&dataqualitymodule;isResultOf">
        <rdfs:comment>inverse property of &#39;involves&#39;.</rdfs:comment>
        <owl:inverseOf rdf:resource="&dataquality;involves"/>
        <rdfs:subPropertyOf rdf:resource="&owl;topObjectProperty"/>
    </owl:ObjectProperty>
    


    <!-- http://www.w3.org/2002/07/owl#topObjectProperty -->

    <owl:ObjectProperty rdf:about="&owl;topObjectProperty"/>
    


    <!-- 
    ///////////////////////////////////////////////////////////////////////////////////////
    //
    // Data properties
    //
    ///////////////////////////////////////////////////////////////////////////////////////
     -->

    


    <!-- http://www.semanticweb.org/ontologies/dataquality.owl#hasValue -->

    <owl:DatatypeProperty rdf:about="&dataquality;hasValue">
        <rdfs:comment>a relation between a service quality observation (or service quality assessment operation) and the result of the service quality assessment operation</rdfs:comment>
        <rdfs:domain rdf:resource="&dataquality;ServiceQualityResult"/>
        <rdfs:range rdf:resource="&xsd;double"/>
        <rdfs:subPropertyOf rdf:resource="&owl;topDataProperty"/>
    </owl:DatatypeProperty>
    


    <!-- http://www.w3.org/2002/07/owl#topDataProperty -->

    <owl:DatatypeProperty rdf:about="&owl;topDataProperty"/>
    


    <!-- 
    ///////////////////////////////////////////////////////////////////////////////////////
    //
    // Classes
    //
    ///////////////////////////////////////////////////////////////////////////////////////
     -->

    


    <!-- http://www.semanticweb.org/ontologies/dataquality.owl#Service -->

    <owl:Class rdf:about="&dataquality;Service">
        <rdfs:comment>A web service</rdfs:comment>
    </owl:Class>
    


    <!-- http://www.semanticweb.org/ontologies/dataquality.owl#ServiceQualityComponent -->

    <owl:Class rdf:about="&dataquality;ServiceQualityComponent">
        <rdfs:comment>A service quality component is any property of the service that the consumer wants to approximate. Examples of service quality components are the reliability or the robustness of the web service. </rdfs:comment>
    </owl:Class>
    


    <!-- http://www.semanticweb.org/ontologies/dataquality.owl#ServiceQualityCriterion -->

    <owl:Class rdf:about="&dataquality;ServiceQualityCriterion">
        <rdfs:comment>A service quality criterion is a criterion defined by the service consumer as meaningful to get information about the quality of the web service. It is a measure that helps to approximate the value of the service quality component.</rdfs:comment>
    </owl:Class>
    


    <!-- http://www.semanticweb.org/ontologies/dataquality.owl#ServiceQualityObservation -->

    <owl:Class rdf:about="&dataquality;ServiceQualityObservation">
        <rdfs:comment>A service quality observation is an operation by which a service quality value is assigned to a service quality component using a (service) quality criterion.  </rdfs:comment>
    </owl:Class>
    


    <!-- http://www.semanticweb.org/ontologies/dataquality.owl#ServiceQualityResult -->

    <owl:Class rdf:about="&dataquality;ServiceQualityResult">
        <rdfs:comment>The result is the outcome of a service quality assessment operation.</rdfs:comment>
    </owl:Class>
</rdf:RDF>



<!-- Generated by the OWL API (version 3.0.0.1469) http://owlapi.sourceforge.net -->

